

# Homework 3

Andrew Hwang

Math 24

Professor Williams

February 3, 2026

## 1 1.6

**Question 14.** Find bases for the following subspaces of  $F^5$ :

$$W_1 = \{(a_1, a_2, a_3, a_4, a_5) \in F^5 : a_1 - a_3 - a_4 = 0\}$$

and

$$W_2 = \{(a_1, a_2, a_3, a_4, a_5) \in F^5 : a_2 = a_3 = a_4, a_1 + a_5 = 0\}.$$

What are the dimensions of  $W_1$  and  $W_2$ ?

*Solution.* Define  $F^5$  as the vector space of 5-tuples over the field  $F$ . First, let us evaluate  $W_1$ . Let  $(a_1, a_2, a_3, a_4, a_5) \in W_1$ . Then the defining condition

$$a_1 - a_3 - a_4 = 0$$

implies

$$a_1 = a_3 + a_4.$$

Hence, every vector in  $W_1$  has the form

$$(a_3 + a_4, a_2, a_3, a_4, a_5).$$

This 5-tuple can be rearranged as a linear combination as such:

$$(a_3 + a_4, a_2, a_3, a_4, a_5) = a_2(0, 1, 0, 0, 0) + a_3(1, 0, 1, 0, 0) + a_4(1, 0, 0, 1, 0) + a_5(0, 0, 0, 0, 1)$$

Let us define set  $\beta_1 = \{(0, 1, 0, 0, 0), (1, 0, 1, 0, 0), (1, 0, 0, 1, 0), (0, 0, 0, 0, 1)\}$ . It is true that  $\beta_1$  spans  $W_1$ . Now, let us show that  $\beta_1$  is linearly independent. Suppose

$$c_1(1, 0, 0, 0, 0) + c_2(0, 1, 0, 0, 0) + c_3(1, 0, 1, 0, 0) + c_4(0, 0, 0, 0, 1) = (0, 0, 0, 0, 0).$$

Then, we get a system of equations

$$\begin{aligned}c_1 + c_3 &= 0, \\c_2 &= 0, \\c_3 &= 0, \\c_4 &= 0.\end{aligned}$$

From  $c_3 = 0$  we get  $c_1 = 0$ , and thus  $c_1 = c_2 = c_3 = c_4 = 0$ . Hence the vectors in  $\beta_1$  are linearly independent. Since  $\beta_1$  spans  $W_1$ , and is linearly independent, it is a basis set for  $W_1$ . Therefore,  $\dim W_1 = 4$ .

Similarly, let  $(a_1, a_2, a_3, a_4, a_5) \in W_2$ . The defining conditions

$$a_2 = a_3 = a_4 \quad \text{and} \quad a_1 + a_5 = 0$$

imply

$$a_1 = -a_5.$$

Hence, every vector in  $W_2$  has the form

$$(-a_5, a_2, a_2, a_2, a_5).$$

Repeating the procedure from evaluating  $W_1$ , we express an arbitrary vector in  $W_2$  as a linear combination:

$$(-a_5, a_2, a_2, a_2, a_5) = a_2(0, 1, 1, 1, 0) + a_5(-1, 0, 0, 0, 1).$$

Thus,  $\beta_2 = \{(0, 1, 1, 1, 0), (-1, 0, 0, 0, 1)\}$  spans  $W_2$ . To show that  $\beta_2$  is linearly independent, assume

$$c_1(0, 1, 1, 1, 0) + c_2(-1, 0, 0, 0, 1) = (0, 0, 0, 0, 0).$$

This gives us a system of equations

$$\begin{aligned}-c_2 &= 0, \\c_1 &= 0, \\c_1 &= 0, \\c_1 &= 0, \\c_2 &= 0.\end{aligned}$$

Hence  $c_1 = c_2 = 0$ , so the vectors in  $\beta_2$  are linearly independent. Therefore,  $\beta_2$  spans  $W_2$  and is linearly independent, so  $\beta_2$  is a basis for  $W_2$ . Thus,  $\dim W_2 = 2$ .

□

**Question 17.** The set of all skew-symmetric  $n \times n$  matrices is a subspace  $W$  of  $M_{n \times n}(F)$ . Find a basis for  $W$ . What is the dimension of  $W$ ?

*Solution.* Let

$$W = \{A \in M_{n \times n}(F) : A^t = -A\}.$$

Comparing each entry in the matrix, the condition  $A^t = -A$  is equivalent to

$$A_{ji} = -A_{ij} \quad \text{for all } i, j.$$

In particular, when  $i = j$  we get  $A_{ii} = -A_{ii}$ , so  $2A_{ii} = 0$ . Hence if  $F$  is not of characteristic 2, then  $A_{ii} = 0$  for all  $i$ .

For each pair  $1 \leq i < j \leq n$ , define

$$K_{ij} = E_{ij} - E_{ji}.$$

Then  $K_{ij}^t = E_{ji} - E_{ij} = -K_{ij}$ , so  $K_{ij} \in W$ . Let  $A = (A_{ij}) \in W$  with  $i < j$ . Since  $A$  is skew-symmetric,  $A_{ji} = -A_{ij}$  and  $A_{ii} = 0$ . Define

$$B = \sum_{1 \leq i < j \leq n} A_{ij} K_{ij}.$$

Then for  $i < j$ , the  $(i, j)$  entry of  $B$  is  $A_{ij}$ , and the  $(j, i)$  entry is  $-A_{ij} = A_{ji}$ . All diagonal entries of  $B$  are zero. Hence  $B$  has the same entries as  $A$ , so  $A = B$ . Therefore, every  $A \in W$  is a linear combination of the matrices  $K_{ij}$ , and

$$W = \text{span}(\{K_{ij} : 1 \leq i < j \leq n\}).$$

Next, we prove that  $\{K_{ij} : 1 \leq i < j \leq n\}$  is linearly independent. Suppose

$$\sum_{1 \leq i < j \leq n} c_{ij} K_{ij} = 0.$$

Fix  $i < j$ . The matrix  $K_{ij}$  is the only basis element with a nonzero entry in the  $(i, j)$  position, where it equals 1. Hence, the  $(i, j)$  entry of the sum equals  $c_{ij}$ . Since the zero matrix has a zero in this position, we obtain  $c_{ij} = 0$  for all  $i < j$ . Therefore, the set is linearly independent, and also a basis set.

To compute  $\dim(W)$ , note that an  $n \times n$  matrix has  $n^2$  entries. In a skew-symmetric matrix  $A^t = -A$ , the diagonal entries satisfy  $A_{ii} = -A_{ii}$ , so  $a_{ii} = 0$  for all  $i$ , giving  $n$  forced zero entries on the diagonal. Among the remaining  $n^2 - n$  off-diagonal entries, the skew-symmetry condition pairs each entry  $(i, j)$  with its mirror  $(j, i)$ , so each pair is determined by a single variable. Thus, the number of free parameters is

$$\frac{n^2 - n}{2} = \frac{n(n-1)}{2}.$$

Hence,

$$\dim(W) = \frac{n(n-1)}{2}.$$

□

**Question 23.** Let  $v_1, v_2, \dots, v_k, v$  be vectors in a vector space  $V$ , and define

$$W_1 = \text{span}(\{v_1, v_2, \dots, v_k\}), \quad W_2 = \text{span}(\{v_1, v_2, \dots, v_k, v\}).$$

- (a) Find necessary and sufficient conditions on  $v$  such that  $\dim(W_1) = \dim(W_2)$ .

**Claim.** Dimensions  $\dim(W_1) = \dim(W_2)$  if and only if  $v \in W_1$ .

*Proof.* In the first direction, assume  $\dim(W_1) = \dim(W_2)$ . Since  $W_1 \subseteq W_2$ , if  $v \notin W_1$  then  $W_1 \subset W_2$ . But proper containment of subspaces forces a strict inequality of dimensions, i.e.  $\dim(W_1) < \dim(W_2)$ , contradicting the assumption. Hence  $v \in W_1$ .

In the other direction, assume  $v \in W_1$ . Then there exist scalars  $a_1, \dots, a_k \in F$  such that

$$v = a_1 v_1 + \dots + a_k v_k.$$

Let  $x \in W_2$  be arbitrary. Then for some scalars  $b_1, \dots, b_k, b \in F$ ,

$$x = b_1 v_1 + \dots + b_k v_k + b v.$$

Substituting the expression for  $v$  gives

$$x = b_1 v_1 + \dots + b_k v_k + b(a_1 v_1 + \dots + a_k v_k) = \sum_{i=1}^k (b_i + b a_i) v_i \in W_1.$$

Thus  $W_2 \subseteq W_1$ . Since  $W_1 \subseteq W_2$ , we have  $W_1 = W_2$ , and therefore  $\dim(W_1) = \dim(W_2)$ . Hence, both directions are proven. □

- (b) State and prove a relationship involving  $\dim(W_1)$  and  $\dim(W_2)$  in the case that  $\dim(W_1) \neq \dim(W_2)$ .

**Claim.** If  $\dim(W_1) \neq \dim(W_2)$ , then  $\dim(W_2) = \dim(W_1) + 1$ .

*Proof.* Assume  $\dim(W_1) \neq \dim(W_2)$ . Since  $W_1 \subseteq W_2$ , we must have

$$\dim(W_1) < \dim(W_2).$$

By part (a),  $\dim(W_1) = \dim(W_2)$  holds exactly when  $v \in W_1$ . Hence  $\dim(W_1) \neq \dim(W_2)$  implies  $v \notin W_1$ .

Let  $B = \{w_1, \dots, w_m\}$  be a basis of  $W_1$ , so  $m = \dim(W_1)$ . We show that  $B \cup \{v\}$  is a basis for  $W_2$ .

First,  $B \cup \{v\}$  spans  $W_2$  because any  $x \in W_2$  can be written as

$$x = y + cv$$

for some  $y \in W_1$  and  $c \in F$  (since  $W_2 = \text{span}(W_1 \cup \{v\})$ ). Because  $B$  spans  $W_1$ , we can write  $y = \sum_{i=1}^m d_i w_i$ , so

$$x = \sum_{i=1}^m d_i w_i + cv \in \text{span}(B \cup \{v\}).$$

Thus  $W_2 \subseteq \text{span}(B \cup \{v\})$ , and the reverse inclusion is immediate from  $B \subseteq W_1 \subseteq W_2$  and  $v \in W_2$ . Hence

$$W_2 = \text{span}(B \cup \{v\}).$$

Next,  $B \cup \{v\}$  is linearly independent. Suppose

$$cv + \sum_{i=1}^m c_i w_i = 0.$$

If  $c \neq 0$ , then

$$v = -\frac{1}{c} \sum_{i=1}^m c_i w_i \in \text{span}(B) = W_1,$$

contradicting  $v \notin W_1$ . Therefore  $c = 0$ , and then  $\sum_{i=1}^m c_i w_i = 0$  implies  $c_1 = \cdots = c_m = 0$  since  $B$  is linearly independent. Hence  $B \cup \{v\}$  is linearly independent.

Basis set  $B$  contains  $\dim(W_1)$  vectors. Adding the vector  $v$  produces a basis for  $W_2$  with one more vector. Hence,

$$\dim(W_2) = \dim(W_1) + 1.$$

□

**Question 33a.** Let  $W_1$  and  $W_2$  be subspaces of a vector space  $V$  such that  $V = W_1 \oplus W_2$ . If  $\beta_1$  and  $\beta_2$  are bases for  $W_1$  and  $W_2$ , respectively, show that  $\beta_1 \cap \beta_2 = \emptyset$  and  $\beta_1 \cup \beta_2$  is a basis for  $V$ .

*Proof.* First, we will prove  $\beta_1 \cap \beta_2 = \emptyset$ . Assume  $\beta_1 \cap \beta_2 \neq \emptyset$ . This means that there is at least one vector  $u$  such that  $u \in \beta_1$  and  $u \in \beta_2$ . Since  $\beta_1$  is a basis for  $W_1$  and  $\beta_2$  is a basis for  $W_2$ , we have  $u \in W_1$  and  $u \in W_2$ , hence  $u \in W_1 \cap W_2$ . Because  $V = W_1 \oplus W_2$ , we know  $W_1 \cap W_2 = \{0\}$ , so  $u = 0$ . This is a contradiction since the zero vector cannot be a basis vector. Therefore  $\beta_1 \cap \beta_2 = \emptyset$ .

Next, we will prove  $\beta_1 \cup \beta_2$  is a basis for  $V$ . To prove  $\beta_1 \cup \beta_2$  is a generating set, let  $v \in V$  be arbitrary. Since  $V = W_1 \oplus W_2$ , we can write

$$v = v_1 + v_2$$

where  $v_1 \in W_1$  and  $v_2 \in W_2$ . Let  $\beta_1 = \{x_1, \dots, x_n\}$  and  $\beta_2 = \{y_1, \dots, y_m\}$ . Since  $\beta_1$  and  $\beta_2$  are bases, there exist scalars  $a_1, \dots, a_n$  and  $b_1, \dots, b_m$  such that

$$v_1 = \sum_{i=1}^n a_i x_i, \quad v_2 = \sum_{j=1}^m b_j y_j.$$

Adding these gives

$$v = v_1 + v_2 = \sum_{i=1}^n a_i x_i + \sum_{j=1}^m b_j y_j,$$

which is a linear combination of vectors from  $\beta_1 \cup \beta_2$ . Hence  $\beta_1 \cup \beta_2$  spans  $V$ .

To prove  $\beta_1 \cup \beta_2$  is linearly independent, suppose

$$\sum_{i=1}^n a_i x_i + \sum_{j=1}^m b_j y_j = 0.$$

Rearranging,

$$\sum_{i=1}^n a_i x_i = - \sum_{j=1}^m b_j y_j.$$

The left-hand side is in  $W_1$ , and the right-hand side is in  $W_2$ . Therefore the common vector lies in  $W_1 \cap W_2$ . Since  $W_1 \cap W_2 = \{0\}$ , it follows that

$$\sum_{i=1}^n a_i x_i = 0 \quad \text{and} \quad \sum_{j=1}^m b_j y_j = 0.$$

Because  $\beta_1$  is linearly independent, we must have  $a_1 = \dots = a_n = 0$ . Because  $\beta_2$  is linearly independent, we must have  $b_1 = \dots = b_m = 0$ . Hence  $\beta_1 \cup \beta_2$  is linearly independent. Since  $\beta_1 \cup \beta_2$  spans  $V$  and is linearly independent, it is a basis for  $V$ .  $\square$

## 2 2.1

**Question 9.** In this exercise,  $T : \mathbb{R}^2 \rightarrow \mathbb{R}^2$  is a function. For each of the following parts, state why  $T$  is not linear.

(a)  $T(a_1 a_2) = (1, a_2)$

*Solution.* Transformation  $T$  does not satisfy the condition  $T(c(a_1, a_2)) = cT(a_1, a_2)$ . Expanding the two sides gives us the following:

$$T(c(a_1, a_2)) = T(ca_1, ca_2) = (1, ca_2),$$

$$cT(a_1, a_2) = c(1, a_2) = (c, ca_2)$$

Since  $(1, ca_2) \neq (c, ca_2)$ ,  $T$  is not linear. □

(b)  $T(a_1 a_2) = (a_1, a_1^2)$

*Solution.* Similarly to part (a),  $T$  does not satisfy the condition  $T(c(a_1, a_2)) = cT(a_1, a_2)$ . Expanding the two sides gives us the following:

$$T(c(a_1, a_2)) = T(ca_1, ca_2) = (ca_1, (ca_1)^2) = (ca_1, c^2 a_1^2),$$

$$cT(a_1, a_2) = c(a_1, a_1^2) = (ca_1, ca_1^2)$$

Since  $(ca_1, c^2 a_1^2) \neq (ca_1, ca_1^2)$ ,  $T$  is not linear. □

(c)  $T(a_1 a_2) = (\sin a_1, 0)$

*Solution.* Transformation  $T$  does not satisfy the condition  $T(a_1 + a_2) = T(a_1) + T(a_2)$ , where  $a_1 = (x_1, y_1)$  and  $a_2 = (x_2, y_2) \in \mathbb{R}^2$ . Expanding both sides gives

$$T(a_1 + a_2) = T(x_1 + x_2, y_1 + y_2) = (\sin(x_1 + x_2), 0)$$

and

$$T(a_1) + T(a_2) = (\sin x_1, 0) + (\sin x_2, 0) = (\sin x_1 + \sin x_2, 0).$$

In general,  $\sin(x_1 + x_2) \neq \sin x_1 + \sin x_2$  (for example, take  $x_1 = x_2 = \frac{\pi}{2}$ ). Hence

$$T(a_1 + a_2) \neq T(a_1) + T(a_2),$$

so  $T$  is not linear. □

**Question 11.** Prove that there exists a linear transformation  $T : \mathbb{R}^2 \rightarrow \mathbb{R}^3$  such that  $T(1, 1) = (1, 0, 2)$  and  $T(2, 3) = (1, -1, 4)$ . What is  $T(8, 11)$ ?

*Proof.* A linear transformation  $T : \mathbb{R}^2 \rightarrow \mathbb{R}^3$  is uniquely determined by its values on a basis of  $\mathbb{R}^2$ . Thus it suffices to show that  $\{(1, 1), (2, 3)\}$  is a basis. The set has two vectors. A linearly independent set of two vectors in  $\mathbb{R}^2$  is automatically a basis, so let us prove the set is linearly independent. Given two scalars  $a, b \in \mathbb{R}$ , evaluate the equation

$$a(1, 1) + b(2, 3) = 0.$$

Expanding the equation as a system of equations gives us

$$a + 2b = 0 \tag{1}$$

$$a + 3b = 0 \tag{2}$$

Subtracting (1) from (2) gives  $b = 0$ , which implies  $a = 0$ . Since the only solution is the trivial one, set  $\{(1, 1), (2, 3)\}$  is linearly independent and hence, a basis set. Therefore, there exists a unique linear transformation  $T$  with such values.

To find  $T(8, 11)$ , note that  $(8, 11)$  can be decomposed into  $2(1, 1) + 3(2, 3)$ . We can use the properties of linear transformations where

$$T(8, 11) = 2T(1, 1) + 3T(2, 3) = 2(1, 0, 2) + 3(1, -1, 4) = (5, -3, 16).$$

□



**Question 17.** Let  $V$  and  $W$  be finite-dimensional vector spaces and  $T : V \rightarrow W$  be linear.

- (a) Prove that if  $\dim(V) < \dim(W)$ , then  $T$  cannot be onto.
- (b) Prove that if  $\dim(V) > \dim(W)$ , then  $T$  cannot be one-to-one.

*Proof.* **(a)** Assume  $\dim(V) < \dim(W)$ . Suppose, for contradiction, that  $T : V \rightarrow W$  is onto. If  $T$  is onto, then  $R(T) = W$ , so

$$\text{rank}(T) = \dim(W).$$

By the Dimension Theorem,

$$\dim(V) = \text{nullity}(T) + \text{rank}(T) = \text{nullity}(T) + \dim(W)$$

However, since  $\text{nullity}(T)$  cannot be negative, this contradicts the assumption  $\dim(V) < \dim(W)$ . Therefore,  $T$  cannot be onto.

**(b)** Assume  $\dim(V) > \dim(W)$ . Suppose, for contradiction, that  $T : V \rightarrow W$  is one-to-one. If  $T$  is one-to-one, then  $\ker(T) = \{0\}$ , so

$$\text{nullity}(T) = 0.$$

Again by the Dimension Theorem,

$$\dim(V) = \text{nullity}(T) + \text{rank}(T) = \text{rank}(T).$$

But  $R(T) \subseteq W$ , so

$$\text{rank}(T) = \dim(R(T)) \leq \dim(W).$$

This contradicts assumption  $\dim(V) > \dim(W)$ . Therefore,  $T$  cannot be one-to-one.  $\square$

**Problem 27.** Using the notation in the definition above, assume that  $T : V \rightarrow V$  is the projection on  $W_1$  to  $W_2$ .

(a) Prove that  $T$  is linear and  $W_1 = \{x \in V : T(x) = x\}$

(b) Prove that  $W_1 = R(T)$  and  $W_2 = N(T)$ .

*Proof.* Assume  $V = W_1 \oplus W_2$ . Then for each  $x \in V$  there exist unique vectors  $x_1 \in W_1$  and  $x_2 \in W_2$  such that  $x = x_1 + x_2$ . Define  $T : V \rightarrow V$  by

$$T(x) = x_1,$$

i.e.,  $T$  is the projection onto  $W_1$  along  $W_2$ .

(a) We first prove that  $T$  is linear. Let  $x, y \in V$  and  $c \in F$ . Write  $x = x_1 + x_2$  and  $y = y_1 + y_2$  with  $x_1, y_1 \in W_1$  and  $x_2, y_2 \in W_2$ . Then

$$cx + y = (cx_1 + y_1) + (cx_2 + y_2),$$

where  $cx_1 + y_1 \in W_1$  and  $cx_2 + y_2 \in W_2$  since  $W_1$  and  $W_2$  are subspaces. By the definition of  $T$ ,

$$T(cx + y) = cx_1 + y_1.$$

On the other hand,

$$cT(x) + T(y) = cx_1 + y_1.$$

Thus  $T(cx + y) = cT(x) + T(y)$ , so  $T$  is linear.

Next we show  $W_1 = \{x \in V : T(x) = x\}$ . If  $x \in W_1$ , then  $x = x + 0$  with  $0 \in W_2$ , so  $T(x) = x$ . Hence  $W_1 \subseteq \{x \in V : T(x) = x\}$ .

Conversely, if  $T(x) = x$ , write  $x = x_1 + x_2$  with  $x_1 \in W_1$ ,  $x_2 \in W_2$ . Then  $T(x) = x_1$ , so  $x_1 = x$ . Hence  $x \in W_1$ . Therefore,

$$W_1 = \{x \in V : T(x) = x\}.$$

(b) We prove  $R(T) = W_1$  and  $N(T) = W_2$ .

First,  $R(T) \subseteq W_1$  because for any  $x \in V$ ,  $T(x) = x_1 \in W_1$ . For the reverse inclusion, let  $w \in W_1$ . Then  $T(w) = w$  by part (a), so  $w \in R(T)$ . Hence  $R(T) = W_1$ .

For the null space, let  $x \in N(T)$ . Write  $x = x_1 + x_2$  with  $x_1 \in W_1$ ,  $x_2 \in W_2$ . Since  $0 = T(x) = x_1$ , we get  $x = x_2 \in W_2$ , so  $N(T) \subseteq W_2$ . Conversely, if  $x_2 \in W_2$ , then  $x_2 = 0 + x_2$  so  $T(x_2) = 0$ , meaning  $x_2 \in N(T)$ . Thus  $W_2 \subseteq N(T)$ , and therefore  $N(T) = W_2$ .  $\square$

### 3 2.2

**Question 4.** Define

$$T : M_{2 \times 2}(\mathbb{R}) \rightarrow P_2(\mathbb{R}) \quad \text{by} \quad T \begin{pmatrix} a & b \\ c & d \end{pmatrix} = (a+b) + (2d)x + bx^2.$$

Let

$$\beta = \left\{ \begin{pmatrix} 1 & 0 \\ 0 & 0 \end{pmatrix}, \begin{pmatrix} 0 & 1 \\ 0 & 0 \end{pmatrix}, \begin{pmatrix} 0 & 0 \\ 1 & 0 \end{pmatrix}, \begin{pmatrix} 0 & 0 \\ 0 & 1 \end{pmatrix} \right\} \quad \text{and} \quad \gamma = \{1, x, x^2\}.$$

Compute  $[T]_{\beta}^{\gamma}$ .

*Solution.* The matrix

$$[T]_{\beta}^{\gamma} = \left[ \left[ T \begin{pmatrix} 1 & 0 \\ 0 & 0 \end{pmatrix} \right]_{\gamma}, \left[ T \begin{pmatrix} 0 & 1 \\ 0 & 0 \end{pmatrix} \right]_{\gamma}, \left[ T \begin{pmatrix} 0 & 0 \\ 1 & 0 \end{pmatrix} \right]_{\gamma}, \left[ T \begin{pmatrix} 0 & 0 \\ 0 & 1 \end{pmatrix} \right]_{\gamma} \right],$$

where  $\beta$  is a basis of  $M_{2 \times 2}(\mathbb{R})$  and  $\gamma$  is a basis of  $P_2(\mathbb{R})$ . Since

$$T \begin{pmatrix} 1 & 0 \\ 0 & 0 \end{pmatrix} = (1+0) + (2(0))x + (0)x^2 = 1,$$

$$T \begin{pmatrix} 0 & 1 \\ 0 & 0 \end{pmatrix} = (0+1) + (2(0))x + (1)x^2 = 1 + x^2,$$

$$T \begin{pmatrix} 0 & 0 \\ 1 & 0 \end{pmatrix} = (0+0) + (2(0))x + (0)x^2 = 0,$$

and

$$T \begin{pmatrix} 0 & 0 \\ 0 & 1 \end{pmatrix} = (0+0) + (2(1))x + (0)x^2 = 2x,$$

we evaluate the coordinate vectors

$$\left[ T \begin{pmatrix} 1 & 0 \\ 0 & 0 \end{pmatrix} \right]_{\gamma} = \begin{pmatrix} 1 \\ 0 \\ 0 \end{pmatrix},$$

$$\left[ T \begin{pmatrix} 0 & 1 \\ 0 & 0 \end{pmatrix} \right]_{\gamma} = \begin{pmatrix} 1 \\ 0 \\ 1 \end{pmatrix},$$

$$\left[ T \begin{pmatrix} 0 & 0 \\ 1 & 0 \end{pmatrix} \right]_{\gamma} = \begin{pmatrix} 0 \\ 0 \\ 0 \end{pmatrix},$$

and

$$\left[ T \begin{pmatrix} 0 & 0 \\ 0 & 1 \end{pmatrix} \right]_{\gamma} = \begin{pmatrix} 0 \\ 2 \\ 0 \end{pmatrix}.$$

Therefore the matrix

$$[T]_{\beta}^{\gamma} = \begin{pmatrix} 1 & 1 & 0 & 0 \\ 0 & 0 & 0 & 2 \\ 0 & 1 & 0 & 0 \end{pmatrix}.$$

□

**Question 8.** Let  $V$  be an  $n$ -dimensional vector space with an ordered basis  $\beta$ . Define  $T : V \rightarrow F^n$  by  $T(x) = [x]_\beta$ . Prove that  $T$  is linear.

*Proof.* Transformation  $T$  is linear if

$$T(cx + y) = cT(x) + T(y),$$

where  $x, y \in V$ . Define an ordered basis  $\beta = \{v_1, v_2, \dots, v_n\}$ . Vectors  $x$  and  $y$  can be expressed as a linear combination of the vectors in the  $\beta$  and scalar  $a_1, a_2, \dots, a_n$  and  $b_1, b_2, \dots, b_n$ , respectively, as

$$x = a_1v_1 + a_2v_2 + \dots + a_nv_n, \quad y = b_1v_1 + b_2v_2 + \dots + b_nv_n.$$

Hence, the transformation is equal to

$$T(x) = [x]_\beta = \begin{pmatrix} a_1 \\ a_2 \\ \vdots \\ a_n \end{pmatrix}, \quad T(y) = [y]_\beta = \begin{pmatrix} b_1 \\ b_2 \\ \vdots \\ b_n \end{pmatrix}.$$

On the left side,  $cx + y$  is equal to

$$cx + y = c(a_1v_1 + a_2v_2 + \dots + a_nv_n) + b_1v_1 + b_2v_2 + \dots + b_nv_n.$$

Factoring results in

$$= (ca_1 + b_1)v_1 + (ca_2 + b_2)v_2 + \dots + (ca_n + b_n)v_n.$$

Hence,

$$T(cx + y) = [cx + y]_\beta = \begin{pmatrix} ca_1 + b_1 \\ ca_2 + b_2 \\ \vdots \\ ca_n + b_n \end{pmatrix}.$$

On the right side,  $cT(x) + T(y)$  expands to

$$cT(x) + T(y) = c[x]_\beta + [y]_\beta = c \begin{pmatrix} a_1 \\ a_2 \\ \vdots \\ a_n \end{pmatrix} + \begin{pmatrix} b_1 \\ b_2 \\ \vdots \\ b_n \end{pmatrix} = \begin{pmatrix} ca_1 + b_1 \\ ca_2 + b_2 \\ \vdots \\ ca_n + b_n \end{pmatrix}.$$

Since both sides are equal, the transformation  $T$  is linear. □

**Question 10.** Let  $V$  be a vector space with the ordered basis  $\beta = \{v_1, v_2, \dots, v_n\}$ . Define  $v_0 = 0$ . By Theorem 2.6, there exist a linear transformation  $T : V \rightarrow V$  such that  $T(v_j) = v_j + v_{j-1}$  for  $j = 1, 2, \dots, n$ . Compute  $[T]_\beta$ .

*Solution.* Let us use the ordered basis is the standard ordered basis  $\beta = \{e_1, e_2, \dots, e_n\}$  to calculate the matrix. Recall that

$$[T]_\beta = [[T(v_1)]_\beta, [T(v_2)]_\beta, \dots, [T(v_n)]_\beta].$$

Next, let us find  $T(v_n)$  for each index  $j \in [1, n]$ :

$$\begin{aligned} T(v_1) &= v_1 + v_0 = e_1, \\ T(v_2) &= v_2 + v_1 = e_2 + e_1, \\ T(v_3) &= v_3 + v_2 = e_3 + e_2, \\ &\vdots \\ T(v_j) &= v_j + v_{j-1} = e_j + e_{j-1}. \end{aligned}$$

Then, the respective column vector  $[T(v_n)]_\beta \in F^n$  is

$$\begin{aligned} [T(v_1)]_\beta &= (1, 0, 0, \dots, 0), \\ [T(v_2)]_\beta &= (1, 1, 0, \dots, 0), \\ [T(v_3)]_\beta &= (0, 1, 1, 0, 0, \dots, 0), \\ &\vdots \\ [T(v_j)]_\beta &= (0, 0, 0, \dots, 1, 1). \end{aligned}$$

Hence, the matrix  $[T]_\beta$  is

$$[T]_\beta = (a_{ij}), \quad a_{ij} = \delta_{ij} + \delta_{i,j-1}.$$

for  $1 \leq i, j \leq n$ . □